Test/Collection/Delta.lean
@@ -31,6 +31,18 @@ def run : IO Unit := do
   assertError "LRX-DELTA-001" 4 3 ((ListDelta.insert 4 9).apply [1, 2, 3])
   assertError "LRX-DELTA-002" 3 3 ((ListDelta.remove 3).apply [1, 2, 3])
   assertError "LRX-DELTA-003" 3 3 ((ListDelta.update 3 9).apply [1, 2, 3])
+  assertError "LRX-DELTA-004" 3 3 ((ListDelta.move 3 0).apply [1, 2, 3])
   assertError "LRX-DELTA-005" 3 2 ((ListDelta.move 0 3).apply [1, 2, 3])
+  assertOk [1, 2, 4, 3] ((ListDelta.insert 3 3).apply [1, 2, 4])
+  assertOk [2, 3, 1] ((ListDelta.move 0 2).apply [1, 2, 3])
+  assertError "LRX-DELTA-002" 0 0 ((ListDelta.remove 0).apply ([] : List Nat))
+  assertError "LRX-DELTA-003" 0 0 ((ListDelta.update 0 1).apply ([] : List Nat))
+  assertError "LRX-DELTA-004" 0 0 ((ListDelta.move 0 0).apply ([] : List Nat))
+  assertError "LRX-DELTA-002" 3 3 <|
+    ListDelta.applyAll [.remove 3, .insert 0 9] [1, 2, 3]
+  let resetThenUpdate := PlannedDeltas.create [0] [2]
+    [.reset #[1], .update 0 2]
+  assertEq true resetThenUpdate.usedReset
+  assertOk [2] (ListDelta.applyAll resetThenUpdate.deltas [0])
 
 end LeanRxTest.Collection.Delta
